% vim:tw=72 sw=2 ft=tex
%         File: thoughts_report.tex
% Date Created: 2013 Jun 18
%  Last Change: 2013 Dec 29
%       Author: hhiker
\documentclass[a4paper]{article}
\usepackage{pdfpages}
\usepackage{xltxtra}
\usepackage{xcolor}
\usepackage{xeCJK}
\usepackage{minted}
\usepackage{booktabs}
\usepackage{amsmath}
\usepackage{paralist}
\usepackage[colorlinks=true,linkcolor=red]{hyperref}
% \usepackage{hyperref}
\usepackage{varioref}
\usepackage{cleveref}
\newcommand{\head}[1]{\textbf{#1}}
\setCJKmainfont[BoldFont=SimHei,ItalicFont=SimSun]{KaiTi}

\newtheorem{theorem}{Theorem}[section]
\newtheorem{lemma}[theorem]{Lemma}
\newtheorem{proposition}[theorem]{Proposition}
\newtheorem{corollary}[theorem]{Corollary}
\newtheorem{definition}{Definition}[section]
\newtheorem{remark}{Remark}[section]

\newenvironment{proof}[1][Proof]{\begin{trivlist}
\item[\hskip \labelsep {\bfseries #1}]}{\end{trivlist}}
\newenvironment{example}[1][Example]{\begin{trivlist}
\item[\hskip \labelsep {\bfseries #1}]}{\end{trivlist}}

\newcommand{\qed}{\nobreak \ifvmode \relax \else
      \ifdim\lastskip<1.5em \hskip-\lastskip
      \hskip1.5em plus0em minus0.5em \fi \nobreak
      \vrule height0.75em width0.5em depth0.25em\fi}

\title{K means within-point scatter deviation\\ \small ——Elements of Statistical
Learning Chapter 14 Reading Note}
\author{Shuai}

\begin{document}
\maketitle

The overall within-point dissimilarity can be replaced with the summation of
dissimilarity between each point in the cluster and the cluster mean, meaning:

\begin{eqnarray}
	W(C) &=& \frac{1}{2}\sum\limits^{K}_{k=1}\sum\limits_{C(i)=k}\sum\limits_{C(i')=k} || x_i - x_{i'} ||^2 \\
	     &=& \sum\limits^{K}_{k=1}N_k\sum\limits_{C(i)=k} || x_i - \bar{x_{k}} ||^2
\end{eqnarray}

where, there are K clusters; $C(i)=k$ means the label given to sample i
is k; $N_k$ means the overall number of points in cluster k; $x_i$ means
sample i.

In this doc, detailed proof will be presented. During the proof, norm will be just written as square.

For expression 1:

For clarity, we replace $\sum\limits_{C(i)=k}\sum\limits_{C(i')=k}$ with $\sum\limits_{i}\sum\limits_{j}$.
\begin{eqnarray}
	\sum\limits_{C(i)=k}\sum\limits_{C(i')=k} || x_i - x_{i'} ||^2 &=&\sum\limits_{i}\sum\limits_{j} || x_i - x_{i'} ||^2\\
	&=& \sum\limits_{i}\sum\limits_{j}(x_i^2 + x_j^2) - \sum\limits_{i}\sum\limits_{j}x_ix_j\\
	&=& N_k\sum\limits_{i}x_i^2 + N_k\sum\limits_{j}x_j^2 - 2\sum\limits_{i}\sum\limits_{j}x_ix_j\\
	&=& 2(N_k\sum\limits_{i}x_i^2 + \sum\limits_{i}\sum\limits_{j}x_ix_j)
\end{eqnarray}

For expression 2:

For clarity, we replace $\sum\limits_{C(i)=k}$ with $\sum\limits_{i}$.
\begin{eqnarray}
	\sum\limits_{C(i)=k} || x_i - \bar{x_{k}} ||^2 &=&\sum\limits_{i} || x_i - \bar{x_{k}} ||^2\\
	&=& \sum\limits_{i}(x_i^2 + \bar{x_k}^2) - \sum\limits_{i}x_i\bar{x_k}\\
	&=& \sum\limits_{i}x_i^2 + N_k\bar{x_k}^2 - \sum\limits_{i}x_i\bar{x_k}\\
	&=& \sum\limits_{i}x_i^2 + N_k\bar{x_k}^2 - 2N_k\bar{x_k}^2\\
	&=& \sum\limits_{i}x_i^2 - N_k\bar{x_k}^2\\
	&=& \sum\limits_{i}x_i^2 - \sum\limits_{i}x_i\sum\limits_{j}x_j/N_k\\
\end{eqnarray}

Since $\sum\limits_{i}x_i\sum\limits_{j}x_j = \sum\limits_{i}\sum\limits_{j}x_ix_j$, proof is done.

\end{document}
